split is_internal spec into is_compat and is_internal + new file for the state monad

theories/Examples/FRP/Memory.v
@@ -86,6 +86,10 @@ Definition tag_of_ref {A : Type} (r : ref A) : Tag :=
 
 Inductive Cell : Type := Cell_ : forall (t : Tag), state t -> Cell.
 
+Definition type_of_cell (c : Cell) :=
+  match c with
+    Cell_ t _ => type_of_tag t
+  end. 
 
 (** ** Concrete memory *)
 
@@ -169,6 +173,38 @@ Proof.
     reflexivity.
 Qed.
 
+Lemma read_update_neq {A : Type} (r : ref A) (v : A) (c : Cell) 
+                      (r' : ref (type_of_cell c)) (mem mem' : Memory) :
+  (id_of_ref r) <> (id_of_ref r') ->
+  read r mem = Some (v,mem') ->
+  read r (id_of_ref r' ↦ c; mem)%pm = Some (v,(id_of_ref r' ↦ c; mem')%pm).
+Proof.
+  unfold read.
+  intros H_neq H_read.
+  destruct (mem (id_of_ref r)) eqn:H_get.
+  - destruct c0,t.
+    -- rewrite p_update_neq; auto.
+       rewrite H_get.
+       destruct (typ_dec T A); subst.
+       + simpl in *.
+         inversion H_read; subst.
+         reflexivity.
+       + inversion H_read.
+    -- rewrite p_update_neq; auto.
+       destruct s;
+       rewrite H_get.
+       + destruct (typ_dec T A); subst.
+         ++ simpl in *.
+            inversion H_read; subst.
+            do 2 f_equal.
+            apply p_update_permute.
+            auto.
+         ++ inversion H_read.
+       + inversion H_read.
+    -- inversion H_read.
+  - inversion H_read. 
+Qed.
+
 (** *** write *)
 
 Definition write {A : Type} (r : ref A) (v : A) (mem : Memory) : option Memory :=
@@ -237,29 +273,35 @@ Proof.
     reflexivity.
 Qed.
 
+(** ** Compatible *)
+
+Definition is_compat {A : Type} (r : ref A) (mem : Memory) :=
+  match mem (id_of_ref r) with
+    | Some (Cell_ (Internal B) _) => B = A 
+    | Some (Cell_ (Input B) (Some _)) => B = A
+    | Some (Cell_ (Output B) None) => B = A
+    | _ => False
+  end.
+
 (** ** being internal *)
 
 Definition is_internal {A : Type} (r : ref A) (mem : Memory) := 
     match mem (id_of_ref r) with
-      | Some (Cell_ (Internal B) _) => B = A
+      | Some (Cell_ (Internal B) _) => True
       | _ => False
     end.
 
 Lemma read_internal_defined : forall (A : Type) (r : ref A) (mem : Memory),
-    is_internal r mem -> read r mem <> None.
+    is_compat r mem -> is_internal r mem -> read r mem <> None.
 Proof.
-  unfold is_internal, read.
-  intros A r mem H_internal.
+  unfold is_compat, is_internal.
+  intros A r mem H_compat H_internal.
   destruct (mem (id_of_ref r)) eqn:H_get.
-  - destruct c, t.
-    -- destruct (typ_dec T A); subst.
-       + intro c.
-         inversion c.
-       + exfalso.
-         apply n.
-         reflexivity.
-    -- contradiction.
-    -- contradiction.
+  - destruct c, t; try contradiction.
+    subst.
+    rewrite (read_internal_spec _ s); auto.
+    intro H_c.
+    inversion H_c.
   - contradiction.
 Qed.
 
@@ -271,94 +313,98 @@ Proof.
   reflexivity.
 Qed.
 
-Lemma read_read_internal (A : Type) (r : ref A) (a : A) (mem mem' : Memory) :
-  is_internal r mem ->
-  read r mem = Some (a, mem') -> mem = mem'.
+Lemma read_none_update_spec {A : Type} (r : ref A) (c : Cell) 
+                            (r' : ref (type_of_cell c)) (mem : Memory) :
+  (id_of_ref r) <> (id_of_ref r') ->
+  read r mem = None -> 
+  read r (((id_of_ref r') ↦ c ; mem)%pm) = None.
 Proof.
-  intros H_internal H_read.
-  destruct (mem (id_of_ref r)) eqn:H_get.
-  - destruct c, t.
-    -- unfold is_internal in H_internal.
-       rewrite H_get in *.
-       subst.
-       rewrite (read_internal_spec _ s) in H_read.
-       + inversion H_read; subst.
-         reflexivity.
-       + simpl.
-         exact H_get.
-    -- unfold is_internal in H_internal.
-       rewrite H_get in *.
-       contradiction.
-    -- unfold is_internal in H_internal.
-       rewrite H_get in *.
-       contradiction.
-  - rewrite read_none_spec in H_read; auto.
+  unfold read.
+  intros H_neq H_read.
+  rewrite p_update_neq; auto.
+  destruct (mem (id_of_ref r)) eqn:H_get; auto.
+  destruct c0,t; auto.
+  - destruct (typ_dec T A); subst; simpl in *; auto.
+    inversion H_read.
+  - destruct s; auto.
+    destruct (typ_dec T A); subst; simpl in *; auto.
     inversion H_read.
 Qed.
 
+Lemma read_read_internal (A : Type) (r : ref A) (a : A) (mem mem' : Memory) :
+  is_compat r mem -> 
+  is_internal r mem ->
+  read r mem = Some (a, mem') -> mem = mem'.
+Proof.
+  unfold is_compat, is_internal.
+  intros H_compat H_internal H_read.
+  destruct (mem (id_of_ref r)) eqn:H_get; 
+  try contradiction.
+  destruct c, t; try contradiction.
+  subst.
+  rewrite (read_internal_spec _ s) in H_read; auto.
+  inversion H_read; subst.
+  reflexivity.
+Qed.
 
 Lemma write_internal_defined : forall (A : Type) (r : ref A) (v : A) (mem : Memory),
-    is_internal r mem -> write r v mem <> None.
+    is_compat r mem -> is_internal r mem -> write r v mem <> None.
 Proof.
-  unfold is_internal, write.
-  intros A r v mem H_internal.
-  destruct (mem (id_of_ref r)) eqn:H_get.
-  - destruct c, t.
-    -- destruct (typ_dec T A); subst.
-       + intro c.
-         inversion c.
-       + exfalso.
-         apply n.
-         reflexivity.
-    -- contradiction.
-    -- contradiction.
-  - contradiction.
+  unfold is_compat, is_internal, write.
+  intros A r v mem H_compat H_internal.
+  destruct (mem (id_of_ref r)) eqn:H_get;
+  try contradiction.
+  destruct c, t; try contradiction.
+  subst.
+  destruct (typ_dec A A).
+  - intro c.
+    inversion c.
+  - exfalso.
+    apply n.
+    reflexivity.
 Qed.
 
 Lemma read_write_internal (A : Type) (r : ref A) (a : A) (mem mem' : Memory) :
+  is_compat r mem -> 
   is_internal r mem ->
   read r mem = Some (a, mem') ->
   write r a mem' = Some mem.
 Proof.
-  intros H_internal H_read.
-  unfold is_internal in *.
-  destruct (mem (id_of_ref r)) eqn:H_get.
-  - destruct c, t; try contradiction.
-    subst.
-    rewrite (read_internal_spec _ s) in H_read; auto.
-    inversion H_read; subst; clear H_read.
-    unfold write.
-    rewrite H_get.
-    destruct (typ_dec A A); subst.
-    -- f_equal.
-       extensionality k.
-       destruct (Nat.eq_dec k (id_of_ref r)) as [| H_neq]; subst.
-       + rewrite p_update_eq.
-         symmetry.
-         exact H_get.
-       + rewrite p_update_neq; auto.
-    -- exfalso.
-       apply n.
-       reflexivity.
-  - contradiction.
+  unfold is_compat, is_internal.
+  intros H_compat H_internal H_read.
+  destruct (mem (id_of_ref r)) eqn:H_get; 
+  try contradiction.
+  destruct c, t; try contradiction.
+  subst.
+  rewrite (read_internal_spec _ s) in H_read; auto.
+  inversion H_read; subst; clear H_read H_internal.
+  rewrite (write_internal_spec _ _ a); auto.
+  f_equal.
+  extensionality k.
+  destruct (Nat.eq_dec k (id_of_ref r)) as [| H_neq]; subst.
+  - rewrite p_update_eq.
+    symmetry.
+    exact H_get.
+  - rewrite p_update_neq; auto.
 Qed.
 
 Lemma write_read_internal (A : Type) (r : ref A) (a : A) (mem mem' : Memory) :
+  is_compat r mem -> 
   is_internal r mem ->
   write r a mem = Some mem' -> 
   read r mem' = Some (a, mem').
 Proof.
-  intros H_internal H_write.
-  unfold is_internal in *.
-  destruct (mem (id_of_ref r)) eqn:H_get.
-  - destruct c,t; try contradiction.
-    subst.
-    rewrite (write_internal_spec _ a s) in H_write; auto.
-    inversion H_write; subst; clear H_write.
-    rewrite (read_internal_spec _ a); auto.
-    rewrite p_update_eq.
-    reflexivity.
-  - contradiction.
+  unfold is_compat, is_internal.
+  intros H_compat H_internal H_write.
+  destruct (mem (id_of_ref r)) eqn:H_get;
+  try contradiction.
+  destruct c,t; try contradiction.
+  subst.
+  rewrite (write_internal_spec _ a s) in H_write; auto.
+  inversion H_write; subst; clear H_write.
+  rewrite (read_internal_spec _ a); auto.
+  rewrite p_update_eq.
+  reflexivity.
 Qed. 
 
 Lemma write_none_spec {A : Type} (r : ref A) (v : A) (mem : Memory) :
@@ -371,387 +417,23 @@ Qed.
 
 
 Lemma write_write_internal (A : Type) (r : ref A) (a a' : A) (mem mem' : Memory) :
+  is_compat r mem ->
   is_internal r mem ->
   write r a mem = Some mem' ->
   write r a' mem = write r a' mem'.
 Proof.
-  intros H_internal H_write.
-  destruct (mem (id_of_ref r)) eqn:H_get.
-  - destruct c, t.
-    -- unfold is_internal in H_internal.
-       rewrite H_get in H_internal; subst.
-       apply (write_internal_spec _ a) in H_get as H_eq.
-       rewrite H_write in *.
-       inversion H_eq; subst; clear H_eq.
-       apply (write_internal_spec _ a') in H_get as H_eq.
-       rewrite H_eq; clear H_eq.
-       rewrite (write_internal_spec _ a' a).
-       + f_equal. 
-         symmetry. 
-         apply p_update_shadow.
-       + now rewrite p_update_eq.
-    -- unfold is_internal in H_internal.
-       rewrite H_get in H_internal.
-       contradiction.
-    -- unfold is_internal in H_internal.
-       rewrite H_get in H_internal.
-       contradiction.
-  - apply (write_none_spec _ a) in H_get.
-    rewrite H_get in *.
-    inversion H_write. 
+  unfold is_compat, is_internal.
+  intros H_compat H_internal H_write.
+  destruct (mem (id_of_ref r)) eqn:H_get; 
+  try contradiction.
+  destruct c, t; try contradiction.
+  subst.
+  rewrite (write_internal_spec _ a s) in H_write; auto.
+  inversion H_write; subst; clear H_write.
+  rewrite (write_internal_spec _ a' s); auto.
+  rewrite (write_internal_spec _ a' a).
+  - f_equal. 
+    symmetry. 
+    apply p_update_shadow.
+  - now rewrite p_update_eq.
 Qed. 
-
-
-
-(** ** State Monad *)
-
-Definition fmap_productLeft {A B X : Type} 
-    (f : A -> B) (p : A * X) : B * X := (f (fst p), snd p).
-
-#[refine] Instance FunctorProductLeft (X : Type) : Functor Typ Typ :=
-{
-    fobj := fun A => A * X;
-    fmap := fun A B => @fmap_productLeft A B X
-}.
-Proof.
--   intros A. extensionality p. destruct p. reflexivity.
--   intros A B C g f. extensionality p. destruct p. reflexivity.
-Defined.
-
-Definition St (A : Type) : Type := Memory -> option (A * Memory).
-
-Definition fmap_St {A B : Type} (f : Typ A B) : St A -> St B  := 
-    fun st => fun m => 
-        (fmap _ ∘ (fmap (FunctorProductLeft Memory))) f (st m).
-
-Lemma functor_prop1 : forall A : Type, fmap_St (idty A) = idty (St A).
-Proof.
-  intro A.
-  unfold fmap_St.
-  extensionality a.
-  extensionality m.
-  simpl.
-  unfold fmap_option.
-  destruct (a m) eqn:H_some; auto.
-  f_equal.
-  unfold fmap_productLeft.
-  destruct p; simpl.
-  reflexivity.
-Qed.
-
-Lemma functor_prop2 :
-forall (A B C : Type) (g : B -> C) (h : A -> B),
-    fmap_St g ∘ fmap_St h = fmap_St (g ∘ h).
-Proof.
-  intros A B C g h.
-  simpl.
-  extensionality a.
-  unfold fmap_St.
-  extensionality m.
-  simpl.
-  destruct (a m) eqn:H_some; auto.
-Qed.
-
-#[refine] Instance Functor_St : Functor Typ Typ := 
-{
-    fobj := St;
-    fmap := @fmap_St;
-}.
-Proof.
-- exact functor_prop1.
-- exact functor_prop2.
-Defined.
-
-Definition ret_st {A : Type} : Typ A (St A) := 
-    fun a m => Some (a, m).
-
-Definition bind_st {A B : Type} (a : St A) (f : A -> St B) : St B :=
-    fun m => match a m with
-    | Some (a, m') => f a m'
-    | None => None
-    end.
-
-Lemma monad_prop1 : 
-  forall (A B : Typ) (f : A -> Functor_St B) (x : A), 
-    bind_st (ret_st x) f = f x.
-Proof.
-  intros A B f x.
-  unfold bind_st.
-  extensionality m.
-  now simpl.
-Qed.
-
-Lemma monad_prop2 : forall (A : Typ) (m : Functor_St A), bind_st m ret_st = m.
-Proof.
-  intros A m.
-  extensionality s.
-  unfold bind_st.
-  destruct (m s) eqn:H_some.
-  - destruct p as [a m'].
-    unfold ret_st.
-    reflexivity.
-  - reflexivity.
-Qed.
-
-Lemma monad_prop3 : forall (A B C : Typ) (m : Functor_St A) (f : A -> Functor_St B)
-    (g : B -> Functor_St C),
-        bind_st (bind_st m f) g = bind_st m (fun x : A => bind_st (f x) g).
-Proof.
-  intros A B C m f g.
-  unfold bind_st.
-  extensionality s.
-  destruct (m s) eqn:H_some.
-  - destruct p as [a s'].
-    reflexivity.
-  - reflexivity.
-Qed.
-
-#[refine] Instance Monad_St : Monad := {
-    ret := @ret_st;
-    bind := @bind_st;
-}.
-Proof.
-- exact monad_prop1.
-- exact monad_prop2.
-- exact monad_prop3.
-Defined.
-
-Definition mget {A : Type} (r : ref A) : St A := read r.
-
-Definition mset {A : Type} (r : ref A) (v : A) : St unit :=
-  fun (m : Memory) => fmap (FunctorOption) (fun (m : Memory) => (tt,m)) (write r v m).
-
-Section st_eq.
-
-  Variables (A : Type).
-  Variables (r : ref A).
-  Variables (x y : A).
-  Variable (σ : Memory).
-
-  Lemma eq_9a : 
-    is_internal r σ ->
-    (mget r >>= (fun _ => mget r)) σ = mget r σ.
-  Proof.
-    intro H_internal.
-    unfold mget; simpl.
-    unfold bind_st; simpl.
-    destruct (read r σ) eqn:H_read.
-    - destruct p as [a σ']. 
-      apply (read_read_internal _ _ _ _ _ H_internal) in H_read as H_eq.
-      subst.
-      exact H_read.
-    -   reflexivity.
-  Qed.
-
-  Lemma eq_9b : 
-    is_internal r σ ->
-    (mget r >>= (mset r)) σ = ret tt σ.
-  Proof.
-    intro H_internal.
-    unfold mget, mset; simpl.
-    unfold bind_st, ret_st; simpl.
-    destruct (read r σ) eqn:H_read.
-    - destruct p as [a σ'].
-      apply (read_read_internal _ _ _ _ _ H_internal) in H_read as H_eq.
-      subst.
-      unfold fmap_option.
-      apply (read_write_internal _ _ _ _ _ H_internal) in H_read.
-      now rewrite H_read.
-    - apply read_internal_defined in H_internal.
-      contradiction.
-  Qed.
-
-  Lemma eq_9c : 
-    is_internal r σ ->
-    (mset r x >>= (fun tt => mget r)) σ = (mset r x >>= (fun tt => ret x)) σ.
-  Proof.
-    intro H_internal.
-    unfold mset, mget; simpl.
-    unfold bind_st, ret_st; simpl.
-    destruct (write r x σ) as [σ'| ] eqn:H_write; simpl.
-    - apply (write_read_internal _ _ _ _ _ H_internal) in H_write.
-      exact H_write.
-    - reflexivity.
-  Qed.
-
-  Lemma eq_9d : 
-    is_internal r σ ->
-    (mset r x >>= (fun tt => mset r y)) σ = (mset r y) σ.
-  Proof.
-    intro H_internal.
-    unfold mset, mget; simpl.
-    unfold bind_st, ret_st; simpl.
-    destruct (write r x σ) as [σ'| ] eqn:H_write; simpl.
-    - unfold fmap_option.
-      destruct (write r y σ) as [σ''| ] eqn:H_write'; simpl.
-      -- rewrite <- (write_write_internal _ _ x _ σ σ'); auto.
-         rewrite H_write'.
-         reflexivity.
-      -- apply (write_internal_defined _ _ y) in H_internal.
-         contradiction.
-    - apply (write_internal_defined _ _ x) in H_internal.
-      contradiction.
-  Qed.
-
-  Lemma eq_9e : 
-    is_internal r σ ->
-    (mget r >>= (fun _ => ret x)) σ = ret x σ.
-  Proof.
-    intro H_internal.
-    unfold mget, ret_st; simpl.
-    unfold bind_st; simpl.
-    destruct (read r σ) as [[a σ'] | ] eqn:Heq.
-    - apply (read_read_internal _ _ _ _ _ H_internal) in Heq.
-      subst.
-      reflexivity.
-    - apply read_internal_defined in H_internal.
-      contradiction.
-  Qed.
-
-End st_eq.
-
-Section st_neq.
-
-    Variables (A B : Type).
-    Variables (r : ref A).
-    Variables (r' : ref B).
-    Variable  (H_neq : id_of_ref r <> id_of_ref r').
-    Variables (x : A) (y : B).
-
-    Lemma eq_9f : 
-      mget r >>= (fun _ => mget r') = mget r' >>= (fun x => mget r >>= (fun _ => ret x)).
-    Proof.
-      unfold mget, ret_st; simpl.
-      unfold bind_st; simpl.
-      unfold read; simpl.
-      extensionality σ.
-      destruct (σ (id_of_ref r)) eqn:H_get.
-      - destruct c, t.
-        -- destruct (typ_dec T A).
-           + destruct (σ (id_of_ref r')) eqn:H_get'; auto.
-             destruct c, t; auto.
-             ++ destruct (typ_dec T0 B); auto.
-                subst.
-                rewrite H_get.
-                destruct (typ_dec A A).
-                * unfold ret_st.
-                  reflexivity.
-                * exfalso.
-                  apply n.
-                  reflexivity.
-             ++ destruct s0; auto.
-                destruct (typ_dec T0 B); auto.
-                subst; simpl.
-                rewrite p_update_neq; auto.
-                rewrite H_get.
-                destruct (typ_dec A A).
-                * unfold ret_st.
-                  reflexivity.
-                * exfalso.
-                  apply n.
-                  reflexivity.
-             + destruct (σ (id_of_ref r')) eqn:H_get'; auto.
-               destruct c, t; auto.
-               ++ destruct (typ_dec T0 B); auto.
-                  subst.
-                  rewrite H_get.
-                  destruct (typ_dec T A).
-                  * contradiction.
-                  * reflexivity.
-               ++ destruct s0; auto.
-                  destruct (typ_dec T0 B); auto.
-                  subst.
-                  simpl.
-                  rewrite p_update_neq; auto.
-                  rewrite H_get.
-                  destruct (typ_dec T A).
-                  * contradiction.
-                  * reflexivity.
-        -- destruct s.
-           + destruct (typ_dec T A).
-             ++ subst.
-                rewrite p_update_neq; auto.
-                destruct (σ (id_of_ref r')) eqn:H_get'; auto.
-                destruct c, t0; auto.
-                * destruct (typ_dec T B); auto.
-                  rewrite H_get.
-                  destruct (typ_dec A A).
-                  ** unfold ret_st.
-                     reflexivity.
-                  ** exfalso.
-                     apply n.
-                     reflexivity.
-                * destruct s; auto.
-                  destruct (typ_dec T B); auto.
-                  subst; simpl.
-                  rewrite p_update_neq; auto.
-                  rewrite H_get.
-                  destruct (typ_dec A A).
-                  ** unfold ret_st.
-                     do 2 f_equal.
-                     now apply p_update_permute.
-                  ** exfalso.
-                     apply n.
-                     reflexivity.
-             ++  destruct (σ (id_of_ref r')) eqn:H_get'; auto.
-                 destruct c, t0; auto.
-                 * destruct (typ_dec T0 B); auto.
-                   subst.
-                   rewrite H_get.
-                   destruct (typ_dec T A); auto.
-                   contradiction.
-                 * destruct s; auto.
-                   destruct (typ_dec T0 B); auto.
-                   rewrite p_update_neq; auto.
-                   rewrite H_get.
-                   destruct (typ_dec T A); auto.
-                   contradiction.
-          + destruct (σ (id_of_ref r')) eqn:H_get'; auto.
-            destruct c, t; auto.
-            ++ destruct (typ_dec T0 B); auto.
-               rewrite H_get.
-               reflexivity.
-            ++ destruct s; auto.
-               destruct (typ_dec T0 B); auto.
-               rewrite p_update_neq; auto.
-               rewrite H_get.
-               reflexivity.
-        -- destruct (σ (id_of_ref r')) eqn:H_get'; auto.
-           destruct c, t; auto.
-           + destruct (typ_dec T0 B); auto.
-             subst.
-             rewrite H_get.
-             reflexivity.
-           + destruct s0; auto.
-             destruct (typ_dec T0 B); auto.
-             rewrite p_update_neq; auto.
-             rewrite H_get.
-             reflexivity.
-      - destruct (σ (id_of_ref r')) eqn:H_get'; auto.
-        destruct c, t; auto.
-        -- destruct (typ_dec T B); auto.
-           subst.
-           rewrite H_get.
-           reflexivity.
-        -- destruct s; auto.
-           destruct (typ_dec T B); auto.
-           rewrite p_update_neq; auto.
-           rewrite H_get.
-           reflexivity.
-    Qed.
-
-    Lemma st_get_set_neq : 
-        mget r >>= (fun _ => mset r' y) = 
-            mset r' y >>= (fun tt => mget r >>= (fun _ => ret tt)).
-    Admitted.
-
-    Lemma st_set_get_neq :
-        mset r x >>= (fun tt => mget r') = 
-            mget r' >>= (fun y => mset r x >>= (fun tt => ret y)).
-    Admitted.
-
-    Lemma st_set_set_neq :
-        mset r x >>= (fun tt => mset r' y) = 
-            mset r' y >>= (fun tt => mset r x).
-    Admitted.
-End st_neq.
